Use notation # instead of ' for literals to avoid conflicts.

barrier/barrier.v
@@ -1,9 +1,9 @@
 From heap_lang Require Export substitution notation.
 
-Definition newbarrier : val := λ: "", ref '0.
-Definition signal : val := λ: "x", "x" <- '1.
+Definition newbarrier : val := λ: "", ref #0.
+Definition signal : val := λ: "x", "x" <- #1.
 Definition wait : val :=
-  rec: "wait" "x" := if: !"x" = '1 then '() else "wait" "x".
+  rec: "wait" "x" := if: !"x" = #1 then #() else "wait" "x".
 
 Instance newbarrier_closed : Closed newbarrier. Proof. solve_closed. Qed.
 Instance signal_closed : Closed signal. Proof. solve_closed. Qed.
