heap_lang/tests.v
@@ -4,20 +4,20 @@ From heap_lang Require Import wp_tactics heap notation.
 Import uPred.
 
 Section LangTests.
-  Definition add := ('21 + '21)%L.
-  Goal ∀ σ, prim_step add σ ('42) σ None.
+  Definition add := (#21 + #21)%L.
+  Goal ∀ σ, prim_step add σ (#42) σ None.
   Proof. intros; do_step done. Qed.
-  Definition rec_app : expr := ((rec: "f" "x" := "f" "x") '0).
+  Definition rec_app : expr := ((rec: "f" "x" := "f" "x") #0).
   Goal ∀ σ, prim_step rec_app σ rec_app σ None.
   Proof.
     intros. rewrite /rec_app. (* FIXME: do_step does not work here *)
-    by eapply (Ectx_step  _ _ _ _ _ []), (BetaS _ _ _ _ '0).
+    by eapply (Ectx_step  _ _ _ _ _ []), (BetaS _ _ _ _ #0).
   Qed.
-  Definition lam : expr := λ: "x", "x" + '21.
-  Goal ∀ σ, prim_step (lam '21)%L σ add σ None.
+  Definition lam : expr := λ: "x", "x" + #21.
+  Goal ∀ σ, prim_step (lam #21)%L σ add σ None.
   Proof.
     intros. rewrite /lam. (* FIXME: do_step does not work here *)
-    by eapply (Ectx_step  _ _ _ _ _ []), (BetaS "" "x" ("x" + '21) _ '21).
+    by eapply (Ectx_step  _ _ _ _ _ []), (BetaS "" "x" ("x" + #21) _ #21).
   Qed.
 End LangTests.
 
@@ -28,9 +28,9 @@ Section LiftingTests.
   Implicit Types Φ : val → iPropG heap_lang Σ.
 
   Definition heap_e  : expr :=
-    let: "x" := ref '1 in "x" <- !"x" + '1;; !"x".
+    let: "x" := ref #1 in "x" <- !"x" + #1;; !"x".
   Lemma heap_e_spec E N :
-     nclose N ⊆ E → heap_ctx N ⊑ || heap_e @ E {{ λ v, v = '2 }}.
+     nclose N ⊆ E → heap_ctx N ⊑ || heap_e @ E {{ λ v, v = #2 }}.
   Proof.
     rewrite /heap_e=>HN. rewrite -(wp_mask_weaken N E) //.
     wp eapply wp_alloc; eauto. apply forall_intro=>l; apply wand_intro_l.
@@ -42,11 +42,11 @@ Section LiftingTests.
 
   Definition FindPred : val :=
     rec: "pred" "x" "y" :=
-      let: "yp" := "y" + '1 in
+      let: "yp" := "y" + #1 in
       if: "yp" < "x" then "pred" "x" "yp" else "y".
   Definition Pred : val :=
     λ: "x",
-      if: "x" ≤ '0 then -FindPred (-"x" + '2) '0 else FindPred "x" '0.
+      if: "x" ≤ #0 then -FindPred (-"x" + #2) #0 else FindPred "x" #0.
 
   Instance FindPred_closed : Closed FindPred | 0.
   Proof. solve_closed. Qed.
@@ -55,7 +55,7 @@ Section LiftingTests.
 
   Lemma FindPred_spec n1 n2 E Φ :
     n1 < n2 → 
-    Φ '(n2 - 1) ⊑ || FindPred 'n2 'n1 @ E {{ Φ }}.
+    Φ #(n2 - 1) ⊑ || FindPred #n2 #n1 @ E {{ Φ }}.
   Proof.
     revert n1. wp_rec=>n1 Hn.
     wp_let. wp_op. wp_let. wp_op=> ?; wp_if.
@@ -64,7 +64,7 @@ Section LiftingTests.
     - assert (n1 = n2 - 1) as -> by omega; auto with I.
   Qed.
 
-  Lemma Pred_spec n E Φ : ▷ Φ (LitV (n - 1)) ⊑ || Pred 'n @ E {{ Φ }}.
+  Lemma Pred_spec n E Φ : ▷ Φ #(n - 1) ⊑ || Pred #n @ E {{ Φ }}.
   Proof.
     wp_lam. wp_op=> ?; wp_if.
     - wp_op. wp_op.
@@ -74,7 +74,7 @@ Section LiftingTests.
   Qed.
 
   Lemma Pred_user E :
-    (True : iProp) ⊑ || let: "x" := Pred '42 in Pred "x" @ E {{ λ v, v = '40 }}.
+    (True : iProp) ⊑ || let: "x" := Pred #42 in Pred "x" @ E {{ λ v, v = #40 }}.
   Proof.
     intros. ewp apply Pred_spec. wp_let. ewp apply Pred_spec. auto with I.
   Qed.
@@ -84,7 +84,7 @@ Section ClosedProofs.
   Definition Σ : rFunctorG := #[ heapGF ].
   Notation iProp := (iPropG heap_lang Σ).
 
-  Lemma heap_e_closed σ : {{ ownP σ : iProp }} heap_e {{ λ v, v = '2 }}.
+  Lemma heap_e_closed σ : {{ ownP σ : iProp }} heap_e {{ λ v, v = #2 }}.
   Proof.
     apply ht_alt. rewrite (heap_alloc ⊤ nroot); last by rewrite nclose_nroot.
     apply wp_strip_pvs, exist_elim=> ?. rewrite and_elim_l.
