barrier/proof.v
@@ -32,7 +32,7 @@ Definition ress (I : gset gname) : iProp :=
   (Π★{set I} (λ i, ∃ R, saved_prop_own i (Next R) ★ ▷ R))%I.
 
 Coercion state_to_val (s : state) : val :=
-  match s with State Low _ => '0 | State High _ => '1 end.
+  match s with State Low _ => #0 | State High _ => #1 end.
 Arguments state_to_val !_ /.
 
 Definition barrier_inv (l : loc) (P : iProp) (s : state) : iProp :=
@@ -126,7 +126,7 @@ Qed.
 Lemma newbarrier_spec (P : iProp) (Φ : val → iProp) :
   heapN ⊥ N →
   (heap_ctx heapN ★ ∀ l, recv l P ★ send l P -★ Φ (LocV l))
-  ⊑ || newbarrier '() {{ Φ }}.
+  ⊑ || newbarrier #() {{ Φ }}.
 Proof.
   intros HN. rewrite /newbarrier. wp_seq.
   rewrite -wp_pvs. wp eapply wp_alloc; eauto with I ndisj.
@@ -140,7 +140,7 @@ Proof.
     ▷ (barrier_inv l P (State Low {[ i ]})) ★ saved_prop_own i (Next P))).
   - rewrite -pvs_intro. cancel [heap_ctx heapN].
     rewrite {1}[saved_prop_own _ _]always_sep_dup. cancel [saved_prop_own i (Next P)].
-    rewrite /barrier_inv /waiting -later_intro. cancel [l ↦ '0]%I.
+    rewrite /barrier_inv /waiting -later_intro. cancel [l ↦ #0]%I.
     rewrite -(exist_intro (const P)) /=. rewrite -[saved_prop_own _ _](left_id True%I (★)%I).
     by rewrite !big_sepS_singleton /= wand_diag -later_intro.
   - rewrite (sts_alloc (barrier_inv l P) ⊤ N); last by eauto.
@@ -172,7 +172,7 @@ Proof.
 Qed.
 
 Lemma signal_spec l P (Φ : val → iProp) :
-  (send l P ★ P ★ Φ '()) ⊑ || signal (LocV l) {{ Φ }}.
+  (send l P ★ P ★ Φ #()) ⊑ || signal (LocV l) {{ Φ }}.
 Proof.
   rewrite /signal /send /barrier_ctx. rewrite sep_exist_r.
   apply exist_elim=>γ. rewrite -!assoc. apply const_elim_sep_l=>?. wp_let.
@@ -183,8 +183,8 @@ Proof.
   apply forall_intro=>-[p I]. apply wand_intro_l. rewrite -!assoc.
   apply const_elim_sep_l=>Hs. destruct p; last done.
   rewrite {1}/barrier_inv =>/={Hs}. rewrite later_sep.
-  eapply wp_store with (v' := '0); eauto with I ndisj. 
-  strip_later. cancel [l ↦ '0]%I.
+  eapply wp_store with (v' := #0); eauto with I ndisj. 
+  strip_later. cancel [l ↦ #0]%I.
   apply wand_intro_l. rewrite -(exist_intro (State High I)).
   rewrite -(exist_intro ∅). rewrite const_equiv /=; last by eauto using signal_step.
   rewrite left_id -later_intro {2}/barrier_inv -!assoc. apply sep_mono_r.
@@ -199,7 +199,7 @@ Proof.
 Qed.
 
 Lemma wait_spec l P (Φ : val → iProp) :
-  (recv l P ★ (P -★ Φ '())) ⊑ || wait (LocV l) {{ Φ }}.
+  (recv l P ★ (P -★ Φ #())) ⊑ || wait (LocV l) {{ Φ }}.
 Proof.
   rename P into R. wp_rec.
   rewrite {1}/recv /barrier_ctx. rewrite !sep_exist_r.
