barrier/specification.v
@@ -12,7 +12,8 @@ Local Notation iProp := (iPropG heap_lang Σ).
 Lemma barrier_spec (heapN N : namespace) :
   heapN ⊥ N →
   ∃ recv send : loc → iProp -n> iProp,
-    (∀ P, heap_ctx heapN ⊑ {{ True }} newbarrier '() {{ λ v, ∃ l, v = LocV l ★ recv l P ★ send l P }}) ∧
+    (∀ P, heap_ctx heapN ⊑ {{ True }} newbarrier #() {{ λ v,
+                             ∃ l : loc, v = LocV l ★ recv l P ★ send l P }}) ∧
     (∀ l P, {{ send l P ★ P }} signal (LocV l) {{ λ _, True }}) ∧
     (∀ l P, {{ recv l P }} wait (LocV l) {{ λ _, P }}) ∧
     (∀ l P Q, recv l (P ★ Q) ={N}=> recv l P ★ recv l Q) ∧
